Ed25519: Point-based programs and separation logic

src/Bedrock/End2End/X25519/EdwardsXYZT.v
@@ -54,96 +54,113 @@ Local Existing Instance field_parameters.
 Local Instance frep25519 : Field.FieldRepresentation := field_representation n Field25519.s c.
 Local Existing Instance frep25519_ok.
 
-Definition add_precomputed := func! (ox, oy, oz, ota, otb, X1, Y1, Z1, Ta1, Tb1, half_ypx, half_ymx, xyd) {
-  stackalloc 40 as YpX1;
-  fe25519_add(YpX1, Y1, X1);
-  stackalloc 40 as YmX1;
-  fe25519_sub(YmX1, Y1, X1);
-  stackalloc 40 as A;
-  fe25519_mul(A, YmX1, half_ymx);
-  stackalloc 40 as B;
-  fe25519_mul(B, YpX1, half_ypx);
-  stackalloc 40 as T1;
-  fe25519_mul(T1, Ta1, Tb1);
-  stackalloc 40 as C;
-  fe25519_mul(C, xyd, T1);
-  fe25519_sub(ota, B, A);
-  stackalloc 40 as F;
-  fe25519_sub(F, Z1, C);
-  stackalloc 40 as G;
-  fe25519_add(G, Z1, C);
-  fe25519_add(otb, B, A);
-  fe25519_mul(ox, ota, F);
-  fe25519_mul(oy, G, otb);
-  fe25519_mul(oz, F, G)
+(* Size of a field element in bytes. This is the same as computing eval in felem_size_bytes, but we want a notation instead of definition. *)
+Local Notation felem_size := 40.
+
+(* Notations help treat curve points like C structs. To avoid notation clashes, projective coordinates are capitalized. *)
+
+(* Member access notation for projective points: (X, Y, Z, Ta, Tb). *)
+Local Notation "A .X" := (expr.op Syntax.bopname.add A (0)) (in custom bedrock_expr at level 2, left associativity, only parsing).
+Local Notation "A .Y" := (expr.op Syntax.bopname.add A (felem_size)) (in custom bedrock_expr at level 2, left associativity, only parsing).
+Local Notation "A .Z" := (expr.op Syntax.bopname.add A (felem_size + felem_size)) (in custom bedrock_expr at level 2, left associativity, only parsing).
+Local Notation "A .Ta" := (expr.op Syntax.bopname.add A (felem_size + felem_size + felem_size)) (in custom bedrock_expr at level 2, left associativity, only parsing).
+Local Notation "A .Tb" := (expr.op Syntax.bopname.add A (felem_size + felem_size + felem_size + felem_size)) (in custom bedrock_expr at level 2, left associativity, only parsing).
+
+(* Member access notation for precomputed points: (half_ypx, half_ymx, xyd). *)
+Local Notation "A .half_ypx" := (expr.op Syntax.bopname.add A (0)) (in custom bedrock_expr at level 2, left associativity, only parsing).
+Local Notation "A .half_ymx" := (expr.op Syntax.bopname.add A (felem_size)) (in custom bedrock_expr at level 2, left associativity, only parsing).
+Local Notation "A .xyd" := (expr.op Syntax.bopname.add A (felem_size + felem_size)) (in custom bedrock_expr at level 2, left associativity, only parsing).
+
+(* Member access notation for cached points: (half_YmX, half_YpX, Z, Td). *)
+Local Notation "A .half_YmX" := (expr.op Syntax.bopname.add A (0)) (in custom bedrock_expr at level 2, left associativity, only parsing).
+Local Notation "A .half_YpX" := (expr.op Syntax.bopname.add A (felem_size)) (in custom bedrock_expr at level 2, left associativity, only parsing).
+Local Notation "A .Z" := (expr.op Syntax.bopname.add A (felem_size + felem_size)) (in custom bedrock_expr at level 2, left associativity, only parsing).
+Local Notation "A .Td" := (expr.op Syntax.bopname.add A (felem_size + felem_size + felem_size)) (in custom bedrock_expr at level 2, left associativity, only parsing).
+
+(* Adds a precomputed point p_b to projective point p_a and puts the result in p_out. *)
+Definition add_precomputed := func! (p_out, p_a, p_b) {
+  stackalloc felem_size as YpX1;
+  fe25519_add(YpX1, p_a.Y, p_a.X);
+  stackalloc felem_size as YmX1;
+  fe25519_sub(YmX1, p_a.Y, p_a.X);
+  stackalloc felem_size as A;
+  fe25519_mul(A, YmX1, p_b.half_ymx);
+  stackalloc felem_size as B;
+  fe25519_mul(B, YpX1, p_b.half_ypx);
+  stackalloc felem_size as T1;
+  fe25519_mul(T1, p_a.Ta, p_a.Tb);
+  stackalloc felem_size as C;
+  fe25519_mul(C, p_b.xyd, T1);
+  fe25519_sub(p_out.Ta, B, A);
+  stackalloc felem_size as F;
+  fe25519_sub(F, p_a.Z, C);
+  stackalloc felem_size as G;
+  fe25519_add(G, p_a.Z, C);
+  fe25519_add(p_out.Tb, B, A);
+  fe25519_mul(p_out.X, p_out.Ta, F);
+  fe25519_mul(p_out.Y, G, p_out.Tb);
+  fe25519_mul(p_out.Z, F, G)
 }.
 
-Definition felem_size := Eval lazy in felem_size_in_bytes.
-
-(* Member access notation for projective points: (x, y, z, ta, tb). *)
-Local Notation "A .x" := (expr.op Syntax.bopname.add A (0)) (in custom bedrock_expr at level 2, left associativity).
-Local Notation "A .y" := (expr.op Syntax.bopname.add A (felem_size)) (in custom bedrock_expr at level 2, left associativity).
-Local Notation "A .z" := (expr.op Syntax.bopname.add A (felem_size + felem_size)) (in custom bedrock_expr at level 2, left associativity).
-Local Notation "A .ta" := (expr.op Syntax.bopname.add A (felem_size + felem_size + felem_size)) (in custom bedrock_expr at level 2, left associativity).
-Local Notation "A .tb" := (expr.op Syntax.bopname.add A (felem_size + felem_size + felem_size + felem_size)) (in custom bedrock_expr at level 2, left associativity).
-
-(* Equivalent of m1double in src/Curves/Edwards/XYZT/Basic.v *)
+(* Doubles a projective point. Equivalent of m1double in src/Curves/Edwards/XYZT/Basic.v *)
 Definition double := func! (p_out, p_a) {
   stackalloc felem_size as trX;
-  fe25519_square(trX, p_a.x);
+  fe25519_square(trX, p_a.X);
   stackalloc felem_size as trZ;
-  fe25519_square(trZ, p_a.y);
+  fe25519_square(trZ, p_a.Y);
   stackalloc felem_size as t0;
-  fe25519_square(t0, p_a.z);
+  fe25519_square(t0, p_a.Z);
   stackalloc felem_size as trT;
   fe25519_carry_add(trT, t0, t0);
   stackalloc felem_size as rY;
-  fe25519_add(rY, p_a.x, p_a.y);
+  fe25519_add(rY, p_a.X, p_a.Y);
   fe25519_square(t0, rY);
-  fe25519_carry_add(p_out.tb, trZ, trX);
+  fe25519_carry_add(p_out.Tb, trZ, trX);
   stackalloc felem_size as cZ;
   fe25519_carry_sub(cZ, trZ, trX);
-  fe25519_sub(p_out.ta, t0, p_out.tb);
+  fe25519_sub(p_out.Ta, t0, p_out.Tb);
   stackalloc felem_size as cT;
   fe25519_sub(cT, trT, cZ);
-  fe25519_mul(p_out.x, p_out.ta, cT);
-  fe25519_mul(p_out.y, p_out.tb, cZ);
-  fe25519_mul(p_out.z, cZ, cT)
+  fe25519_mul(p_out.X, p_out.Ta, cT);
+  fe25519_mul(p_out.Y, p_out.Tb, cZ);
+  fe25519_mul(p_out.Z, cZ, cT)
 }.
 
-(* Converting a normal point to a cached point to prepare it for readdition. *)
-Definition to_cached := func! (ohalf_ymx, ohalf_ypx, oz, otd, x, y, z, ta, tb, d) {
-  fe25519_sub(ohalf_ymx, y, x);
-  fe25519_half(ohalf_ymx, ohalf_ymx); (* This doesn't exist yet, work with spec for now. *)
-  fe25519_add(ohalf_ypx, y, x);
-  fe25519_half(ohalf_ypx, ohalf_ypx);
-  fe25519_mul(otd, ta, tb);
-  fe25519_mul(otd, otd, d);
-  fe25519_copy(oz, z)
+(* Converts a projective point p_a to a cached point p_out to prepare it for readdition. 
+   Uses the field's parameter d, which is passed as p_d for now. *)
+Definition to_cached := func! (p_out, p_a, p_d) {
+  fe25519_sub(p_out.half_YmX, p_a.Y, p_a.X);
+  fe25519_half(p_out.half_YmX, p_out.half_YmX); (* An implementation doesn't exist yet, work with spec for now. *)
+  fe25519_add(p_out.half_YpX, p_a.Y, p_a.X);
+  fe25519_half(p_out.half_YpX, p_out.half_YpX);
+  fe25519_mul(p_out.Td, p_a.Ta, p_a.Tb);
+  fe25519_mul(p_out.Td, p_out.Td, p_d);
+  fe25519_copy(p_out.Z, p_a.Z)
 }.
 
-(* Equivalent of m1_readd in src/Curves/Edwards/XYZT/Readdition.v *)
-Definition readd := func! (ox, oy, oz, ota, otb, X1, Y1, Z1, Ta1, Tb1, half_YmX, half_YpX, Z2, Td) {
-  stackalloc 40 as A;
-  fe25519_sub(A, Y1, X1);
-  fe25519_mul(A, A, half_YmX);
-  stackalloc 40 as B;
-  fe25519_add(B, Y1, X1);
-  fe25519_mul(B, B, half_YpX);
-  stackalloc 40 as C;
-  fe25519_mul(C, Ta1, Tb1);
-  fe25519_mul(C, C, Td);
-  stackalloc 40 as D;
-  fe25519_mul(D, Z1, Z2);
-  fe25519_sub(ota, B, A);
-  stackalloc 40 as F;
+(* Equivalent of m1_readd in src/Curves/Edwards/XYZT/Readdition.v 
+   Adds a projective point p_a and cached point p_c and stores the result as projective point in p_out. *)
+Definition readd := func! (p_out, p_a, p_c) {
+  stackalloc felem_size as A;
+  fe25519_sub(A, p_a.Y, p_a.X);
+  fe25519_mul(A, A, p_c.half_YmX);
+  stackalloc felem_size as B;
+  fe25519_add(B, p_a.Y, p_a.X);
+  fe25519_mul(B, B, p_c.half_YpX);
+  stackalloc felem_size as C;
+  fe25519_mul(C, p_a.Ta, p_a.Tb);
+  fe25519_mul(C, C, p_c.Td);
+  stackalloc felem_size as D;
+  fe25519_mul(D, p_a.Z, p_c.Z);
+  fe25519_sub(p_out.Ta, B, A);
+  stackalloc felem_size as F;
   fe25519_sub(F, D, C);
-  stackalloc 40 as G;
+  stackalloc felem_size as G;
   fe25519_add(G, D, C);
-  fe25519_add(otb, B, A);
-  fe25519_mul(ox, ota, F);
-  fe25519_mul(oy, G, otb);
-  fe25519_mul(oz, F, G)
+  fe25519_add(p_out.Tb, B, A);
+  fe25519_mul(p_out.X, p_out.Ta, F);
+  fe25519_mul(p_out.Y, G, p_out.Tb);
+  fe25519_mul(p_out.Z, F, G)
 }.
 
 Section WithParameters.
@@ -165,7 +182,9 @@ Local Notation word := (Naive.word 32).
 Local Notation felem := (felem(FieldRepresentation:=frep25519)).
 Local Notation point := (point(Feq:=Logic.eq)(Fzero:=F.zero)(Fadd:=F.add)(Fmul:=F.mul)(a:=a)(d:=d)).
 Local Notation cached := (cached(Fzero:=F.zero)(Fadd:=F.add)(Fmul:=F.mul)(a:=a)(d:=d)).
-Local Notation coordinates := (coordinates(Feq:=Logic.eq)).
+Local Notation coordinates := (coordinates(Fzero:=F.zero)(Fadd:=F.add)(Fmul:=F.mul)(Feq:=Logic.eq)(a:=a)(d:=d)).
+Local Notation cached_coordinates := (cached_coordinates(Fzero:=F.zero)(Fadd:=F.add)(Fdiv:=F.div)(Fmul:=F.mul)(Fsub:=F.sub)(Feq:=Logic.eq)(a:=a)(d:=d)).
+Local Notation precomputed_coordinates := (precomputed_coordinates(Fone:=F.one)(Fadd:=F.add)(Fmul:=F.mul)(Fsub:=F.sub)(Feq:=Logic.eq)(a:=a)(d:=d)).
 Local Notation m1double :=
   (m1double(F:=F M_pos)(Feq:=Logic.eq)(Fzero:=F.zero)(Fone:=F.one)
            (Fopp:=F.opp)(Fadd:=F.add)(Fsub:=F.sub)(Fmul:=F.mul)(Finv:=F.inv)(Fdiv:=F.div)
@@ -191,6 +210,29 @@ Local Notation m1add_precomputed_coordinates :=
            (a:=a)(d:=d)(nonzero_a:=nonzero_a)(square_a:=square_a)(nonsquare_d:=nonsquare_d)
            (a_eq_minus1:=a_eq_minus1)).
 
+Local Notation "p .+ n" := (word.add p (word.of_Z n)) (at level 50, format "p .+ n", left associativity).
+
+Definition projective_repr P := { p | let '(x,y,z,ta,tb) := p in
+                            coordinates P = (feval x, feval y, feval z, feval ta, feval tb) /\
+                            bounded_by tight_bounds x /\ bounded_by tight_bounds y /\ bounded_by tight_bounds z /\
+                              bounded_by loose_bounds ta /\ bounded_by loose_bounds tb }.
+Local Notation "c 'p5@' p" := (let '(x,y,z,ta,tb) := proj1_sig c in sep (sep (sep (sep (FElem (p .+ 0) x) (FElem (p .+ felem_size) y)) 
+                              (FElem (p .+ (felem_size + felem_size)) z)) (FElem (p .+ (felem_size + felem_size + felem_size)) ta))
+                              (FElem (p .+ (felem_size + felem_size + felem_size + felem_size)) tb)) (at level 10, format "c 'p5@' p").
+
+
+Definition precomputed_repr (P : precomputed_point) := { p | let '(half_ymx, half_ypx, xyd) := p in
+                            precomputed_coordinates P = (feval half_ymx, feval half_ypx, feval xyd) /\
+                            bounded_by loose_bounds half_ymx /\ bounded_by loose_bounds half_ypx /\ bounded_by loose_bounds xyd }.
+Local Notation "c 'p3@' p" := (let '(half_ymx, half_ypx, xyd) := proj1_sig c in sep (sep (FElem (p .+ 0) half_ymx) (FElem (p .+ felem_size) half_ypx))
+                              (FElem (p .+ (felem_size + felem_size)) xyd)) (at level 10, format "c 'p3@' p").
+
+Definition cached_repr (P : cached) := { p | let '(half_ymx, half_ypx,z,td) := p in
+                            cached_coordinates P = (feval half_ymx, feval half_ypx, feval z, feval td) /\
+                            bounded_by loose_bounds half_ymx /\ bounded_by loose_bounds half_ypx /\bounded_by loose_bounds z /\ bounded_by loose_bounds td }.
+Local Notation "c 'p4@' p" := (let '(half_ymx, half_ypx,z,td) := proj1_sig c in sep (sep (sep (FElem (p .+ 0) half_ymx) (FElem (p .+ felem_size) half_ypx))
+                              (FElem (p .+ (felem_size + felem_size)) z)) (FElem (p .+ (felem_size + felem_size + felem_size)) td)) (at level 10, format "c 'p4@' p").
+
 Instance spec_of_fe25519_half : spec_of "fe25519_half" :=
   fnspec! "fe25519_half"
     (result_location input_location: word) / (old_result input: felem)
@@ -206,117 +248,56 @@ Instance spec_of_fe25519_half : spec_of "fe25519_half" :=
         feval result = F.div (feval input) (F.add F.one F.one) /\
         m' =* (FElem result_location result)  * R}.
 
+(* TODO: Use anybytes or similar for output pointer preconditions once the field operation preconditions are suffiently weakened. *)
+
 Global Instance spec_of_add_precomputed : spec_of "add_precomputed" :=
   fnspec! "add_precomputed"
-    (oxK oyK ozK otaK otbK X1K Y1K Z1K Ta1K Tb1K half_ypxK half_ymxK xydK : word) /
-    (ox oy oz ota otb X1 Y1 Z1 Ta1 Tb1 half_ypx half_ymx xyd : felem) (p : point) (c: precomputed_point) (R : _ -> Prop),
-  { requires t m :=
-      coordinates p = ((feval X1), (feval Y1), (feval Z1), (feval Ta1), (feval Tb1)) /\
-      precomputed_coordinates c = ((feval half_ypx), (feval half_ymx), (feval xyd)) /\
-      bounded_by tight_bounds X1 /\
-      bounded_by tight_bounds Y1 /\
-      bounded_by tight_bounds Z1 /\
-      bounded_by loose_bounds Ta1 /\
-      bounded_by loose_bounds Tb1 /\
-      bounded_by loose_bounds half_ypx /\
-      bounded_by loose_bounds half_ymx /\
-      bounded_by loose_bounds xyd /\
-      m =* (FElem X1K X1) * (FElem Y1K Y1) * (FElem Z1K Z1) * (FElem Ta1K Ta1) * (FElem Tb1K Tb1) * (FElem half_ypxK half_ypx) * (FElem half_ymxK half_ymx) * (FElem xydK xyd) * (FElem oxK ox) * (FElem oyK oy) * (FElem ozK oz) * (FElem otaK ota) * (FElem otbK otb) * R;
-    ensures t' m' :=
-      t = t' /\
-      exists ox' oy' oz' ota' otb',
-        ((feval ox'), (feval oy'), (feval oz'), (feval ota'), (feval otb')) = 
-            coordinates (m1add_precomputed_coordinates p c) /\
-        bounded_by loose_bounds ox' /\
-        bounded_by loose_bounds oy' /\
-        bounded_by loose_bounds oz' /\
-        bounded_by loose_bounds ota' /\
-        bounded_by loose_bounds otb' /\
-        m' =* (FElem X1K X1) * (FElem Y1K Y1) * (FElem Z1K Z1) * (FElem Ta1K Ta1) * (FElem Tb1K Tb1) * (FElem half_ypxK half_ypx) * (FElem half_ymxK half_ymx) * (FElem xydK xyd) * (FElem oxK ox') * (FElem oyK oy') * (FElem ozK oz') * (FElem otaK ota') * (FElem otbK otb') * R }.
-
-Definition point_repr_bounds := (Field.bounds * Field.bounds * Field.bounds * Field.bounds * Field.bounds)%type.
-Definition point_repr := (felem * felem * felem * felem * felem)%type.
-Definition feval_point_repr '(x, y, z, ta, tb) := (feval x, feval y, feval z, feval ta, feval tb).
-
-Definition point_repr_bounded_by (bounds : point_repr_bounds) '(x,y,z,ta,tb) : Prop :=
-  let '(bounds_x, bounds_y, bounds_z, bounds_ta, bounds_tb) := bounds in
-  bounded_by bounds_x x /\ bounded_by bounds_y y /\ bounded_by bounds_z z /\ bounded_by bounds_ta ta /\ bounded_by bounds_tb tb.
-
-Local Notation "p .+ n" := (word.add p (word.of_Z n)) (at level 50, format "p .+ n", left associativity).
-Local Notation "c p@ p" := (let '(x,y,z,ta,tb) := c in sep (sep (sep (sep (FElem (p .+ 0) x) (FElem (p .+ 40) y)) (FElem (p .+ 80) z)) (FElem (p .+ 120) ta)) (FElem (p .+ 160) tb)) (at level 10, format "c p@ p").
+    (p_out p_a p_b: word) / (a any: point) (b: precomputed_point) (a_repr: projective_repr a) (b_repr: precomputed_repr b) (anything: projective_repr any) (R: _ -> Prop), {
+      requires t m :=
+        m =* anything p5@ p_out * a_repr p5@ p_a * b_repr p3@ p_b * R; 
+      ensures t' m' :=
+        t = t' /\
+        exists a_plus_b : projective_repr (m1add_precomputed_coordinates a b),
+          m' =* a_plus_b p5@ p_out * a_repr p5@ p_a * b_repr p3@ p_b * R
+    }.
 
 Global Instance spec_of_double : spec_of "double" :=
   fnspec! "double"
-    (p_out p_a : word) /
-    (p : point) (a anything: point_repr) (R : _ -> Prop), {
-    requires t m :=
-      m =* anything p@ p_out * a p@ p_a * R /\
-      feval_point_repr a = coordinates p /\
-      point_repr_bounded_by (tight_bounds, tight_bounds, loose_bounds, loose_bounds, loose_bounds) a;
-    ensures t' m' := 
-      t = t' /\
-      exists a_double : point_repr,
-      m' =* a_double p@ p_out * a p@ p_a * R /\
-      coordinates (@m1double p) = feval_point_repr a_double /\
-      point_repr_bounded_by (tight_bounds, tight_bounds, tight_bounds, loose_bounds, tight_bounds) a_double
-  }.
+    (p_out p_a: word) /
+    (a any: point) (a_repr: projective_repr a) (anything: projective_repr any) (R: _ -> Prop), {
+      requires t m :=
+        m =* anything p5@ p_out * a_repr p5@ p_a * R;
+      ensures t' m' := 
+        t = t' /\
+        exists a_double: projective_repr (m1double a),
+          m' =* a_double p5@ p_out * a_repr p5@ p_a * R
+    }.
 
 Global Instance spec_of_to_cached: spec_of "to_cached" :=
   fnspec! "to_cached"
-    (ohalf_ymxK ohalf_ypxK ozK otdK xK yK zK taK tbK dK : word) /
-    (ohalf_ymx ohalf_ypx oz otd x y z ta tb d1 : felem) (p: point) (R: _ -> Prop),
-  { requires t m :=
-      coordinates p = ((feval x), (feval y), (feval z), (feval ta), (feval tb)) /\
-      d = (feval d1) /\
-      bounded_by tight_bounds x /\
-      bounded_by tight_bounds y /\
-      bounded_by tight_bounds z /\
-      bounded_by tight_bounds ta /\
-      bounded_by tight_bounds tb /\
-      bounded_by tight_bounds d1 /\
-      m =* (FElem xK x) * (FElem yK y) * (FElem zK z) * (FElem taK ta) * (FElem tbK tb) *
-           (FElem ohalf_ymxK ohalf_ymx) * (FElem ohalf_ypxK ohalf_ypx) * (FElem ozK oz) * (FElem otdK otd) *
-           (FElem dK d1) * R;
-    ensures t' m' :=
-      t = t' /\
-     exists ohalf_ymx' ohalf_ypx' oz' otd',
-       cached_coordinates (@m1_prep p) = ((feval ohalf_ymx'), (feval ohalf_ypx'), (feval oz'), (feval otd')) /\
-       bounded_by tight_bounds ohalf_ymx' /\
-       bounded_by tight_bounds ohalf_ypx' /\
-       bounded_by tight_bounds oz' /\
-       bounded_by tight_bounds otd' /\
-       m' =* (FElem xK x) * (FElem yK y) * (FElem zK z) * (FElem taK ta) * (FElem tbK tb) *
-             (FElem ohalf_ymxK ohalf_ymx') * (FElem ohalf_ypxK ohalf_ypx') * (FElem ozK oz') * (FElem otdK otd') *
-             (FElem dK d1) * R }.
+    (p_out p_a p_d: word) /
+    (a: point) (any: cached) (a_repr: projective_repr a) (anything: cached_repr any) (d1: felem) (R: _ -> Prop), {
+      requires t m :=
+        m =* anything p4@ p_out * a_repr p5@ p_a * FElem p_d d1 * R /\
+        d = feval d1 /\
+        bounded_by tight_bounds d1;
+      ensures t' m' :=
+        t = t' /\
+        exists a_cached: cached_repr (m1_prep a),
+          m' =* a_cached p4@ p_out * a_repr p5@ p_a * FElem p_d d1 * R
+  }.
 
 Global Instance spec_of_readd : spec_of "readd" :=
   fnspec! "readd"
-    ( oxK oyK ozK otaK otbK X1K Y1K Z1K Ta1K Tb1K half_YmXK half_YpXK Z2K TdK : word) /
-    ( ox oy oz ota otb X1 Y1 Z1 Ta1 Tb1 half_YmX half_YpX Z2 Td : felem) (p : point) (c: cached) (R : _ -> Prop),
-  { requires t m :=
-      coordinates p = ((feval X1), (feval Y1), (feval Z1), (feval Ta1), (feval Tb1)) /\
-      bounded_by tight_bounds X1 /\
-      bounded_by tight_bounds Y1 /\
-      bounded_by tight_bounds Z1 /\
-      bounded_by loose_bounds Ta1 /\
-      bounded_by loose_bounds Tb1 /\
-      cached_coordinates c = ((feval half_YmX), (feval half_YpX), (feval Z2), (feval Td)) /\
-      bounded_by loose_bounds half_YmX /\
-      bounded_by loose_bounds half_YpX /\
-      bounded_by loose_bounds Z2 /\
-      bounded_by loose_bounds Td /\
-      m =* (FElem X1K X1) * (FElem Y1K Y1) * (FElem Z1K Z1) * (FElem Ta1K Ta1) * (FElem Tb1K Tb1) * (FElem half_YmXK half_YmX) * (FElem half_YpXK half_YpX) * (FElem Z2K Z2) * (FElem TdK Td) * (FElem oxK ox) * (FElem oyK oy) * (FElem ozK oz) * (FElem otaK ota) * (FElem otbK otb) * R;
-    ensures t' m' :=
-      t = t' /\
-      exists ox' oy' oz' ota' otb',
-        ((feval ox'), (feval oy'), (feval oz'), (feval ota'), (feval otb')) = coordinates (@m1_readd p c)/\
-        bounded_by tight_bounds ox' /\
-        bounded_by tight_bounds oy' /\
-        bounded_by tight_bounds oz' /\
-        bounded_by loose_bounds ota' /\
-        bounded_by loose_bounds otb' /\
-        m' =*(FElem X1K X1) * (FElem Y1K Y1) * (FElem Z1K Z1) * (FElem Ta1K Ta1) * (FElem Tb1K Tb1) * (FElem half_YmXK half_YmX) * (FElem half_YpXK half_YpX) * (FElem Z2K Z2) * (FElem TdK Td)* (FElem oxK ox') * (FElem oyK oy') * (FElem ozK oz') * (FElem otaK ota') * (FElem otbK otb') * R }.
-
+    (p_out p_a p_c: word) /
+    (a any: point) (c: cached) (a_repr: projective_repr a) (anything: projective_repr any) (c_repr: cached_repr c) (R : _ -> Prop), {
+      requires t m :=
+        m =* anything p5@ p_out * a_repr p5@ p_a * c_repr p4@ p_c * R;
+      ensures t' m' :=
+        t = t' /\
+        exists a_plus_c: projective_repr (m1_readd a c),
+          m' =* a_plus_c p5@ p_out * a_repr p5@ p_a * c_repr p4@ p_c * R
+    }.
 
 Local Instance spec_of_fe25519_square : spec_of "fe25519_square" := Field.spec_of_UnOp un_square.
 Local Instance spec_of_fe25519_mul : spec_of "fe25519_mul" := Field.spec_of_BinOp bin_mul.
@@ -335,9 +316,22 @@ Local Arguments word.add : simpl never.
 
 Local Arguments feval : simpl never.
 
+Local Ltac destruct_points :=
+  repeat match goal with
+    | _ => progress destruct_head' @Readdition.cached
+    | _ => progress destruct_head' cached_repr
+    | _ => progress destruct_head' @Basic.point
+    | _ => progress destruct_head' projective_repr
+    | _ => progress destruct_head' @precomputed_point
+    | _ => progress destruct_head' precomputed_repr
+    | _ => progress destruct_head' prod
+    | _ => progress destruct_head' and
+    | _ => progress lazy beta match zeta delta [coordinates precomputed_coordinates cached_coordinates proj1_sig] in *
+  end.
+
 Local Ltac cbv_bounds H :=
-  cbv [point_repr_bounded_by un_xbounds bin_xbounds bin_ybounds un_square bin_mul bin_add bin_carry_add bin_sub bin_carry_sub un_outbounds bin_outbounds] in H;
-  cbv [point_repr_bounded_by un_xbounds bin_xbounds bin_ybounds un_square bin_mul bin_add bin_carry_add bin_sub bin_carry_sub un_outbounds bin_outbounds].
+  cbv [un_xbounds bin_xbounds bin_ybounds un_square bin_mul bin_add bin_carry_add bin_sub bin_carry_sub un_outbounds bin_outbounds] in H;
+  cbv [un_xbounds bin_xbounds bin_ybounds un_square bin_mul bin_add bin_carry_add bin_sub bin_carry_sub un_outbounds bin_outbounds].
 
 Local Ltac solve_bounds :=
   repeat match goal with
@@ -351,6 +345,21 @@ Local Ltac solve_mem :=
   repeat match goal with
   | |- exists _ : _ -> Prop, _%sep _ => eexists
   | |- _%sep _ => ecancel_assumption
+  | |- context[?a + ?b] => match isZcst a with 
+        | false => fail
+        | true => match (isZcst b) with
+            | false => fail
+            | true => let c := eval cbv in (a + b) in change (a + b) with c (* Simplify addition of constants. *)
+          end
+      end
+  | H: ?P%sep _ |- _ => match P with context[?a + ?b] => match isZcst a with 
+          | false => fail
+          | true => match (isZcst b) with
+              | false => fail
+              | true => let c := eval cbv in (a + b) in change (a + b) with c in H
+          end
+        end 
+      end
   end.
 
 Local Ltac solve_stack :=
@@ -416,55 +425,43 @@ Proof.
   reflexivity. (* ...and completes immediately *)
 Qed.
 
+Lemma to_cached_ok: program_logic_goal_for_function! to_cached.
+Proof.
+  (* Without this, resolution of cbv stalls out Qed. *)
+  Strategy -1000 [un_xbounds bin_xbounds bin_ybounds un_square bin_mul bin_add bin_carry_add bin_sub bin_carry_sub un_outbounds bin_outbounds].
+
+  straightline.
+  destruct_points.
+
+  repeat single_step.
+  repeat straightline.
+
+  lazy delta [cached_repr].
+  unshelve eexists.
+  eexists (_, _, _, _). 2: solve_mem.
+  lazy match zeta beta delta [bin_model bin_mul bin_add bin_carry_add bin_sub cached_coordinates coordinates proj1_sig m1_prep] in *.
+  ssplit; try solve_bounds.
+  congruence.
+Qed.
+
 Lemma add_precomputed_ok : program_logic_goal_for_function! add_precomputed.
 Proof.
   (* Without this, resolution of cbv stalls out Qed. *)
   Strategy -1000 [un_xbounds bin_xbounds bin_ybounds un_square bin_mul bin_add bin_carry_add bin_sub un_outbounds bin_outbounds].
 
-  (* Unwrap each call in the program. *)
-  (* Each binop produces 2 memory goals on the inputs, 2 bounds goals on the inputs, and 1 memory goal on the output. *)
-  single_step. (* fe25519_add(YpX1, Y1, X1) *)
-  single_step. (* fe25519_sub(YmX1, Y1, X1) *)
-  single_step. (* fe25519_mul(A, YmX1, half_ymx) *)
-  single_step. (* fe25519_mul(B, YpX1, half_ypx) *)
-  single_step. (* fe25519_mul(T1, Ta1, Tb1) *)
-  single_step. (* fe25519_mul(C, xyd, T1) *)
-  single_step. (* fe25519_sub(ota, B, A) *)
-  single_step. (* fe25519_sub(F, Z1, C) *)
-  single_step. (* fe25519_add(G, Z1, C) *)
-  single_step. (* fe25519_add(otb, B, A) *)
-  single_step. (* fe25519_mul(ox, ota, F) *)
-  single_step. (* fe25519_mul(oy, G, otb) *)
-  single_step. (* fe25519_mul(oz, F, G) *)
-
-  (* Solve the postconditions *)
   repeat straightline.
-  (* Rewrites the FElems for the stack (in H93) to be about bytes instead *)
-    cbv [FElem] in *.
-    (* Prevent output from being rewritten by seprewrite_in *)
-    remember (Bignum.Bignum felem_size_in_words ozK _) as Pz in H95.
-    remember (Bignum.Bignum felem_size_in_words oyK _) as Py in H95.
-    remember (Bignum.Bignum felem_size_in_words oxK _) as Px in H95.
-    remember (Bignum.Bignum felem_size_in_words otbK _) as Ptb in H95.
-    remember (Bignum.Bignum felem_size_in_words otaK _) as Pta in H95.
-    do 8 (seprewrite_in @Bignum.Bignum_to_bytes H95).
-    subst Pz Py Px Ptb Pta.
-    extract_ex1_and_emp_in H95.
+  destruct_points.
 
-  (* Solve stack/memory stuff *)
+  repeat single_step.
   repeat straightline.
+  solve_deallocation.
 
-  (* Post-conditions *)
-  exists x9,x10,x11,x5,x8; ssplit. 2,3,4,5,6:solve_bounds.
-  { (* Correctness: result matches Gallina *)
-    destruct p, c.
-    lazy [bin_model bin_mul bin_add bin_carry_add bin_sub coordinates proj1_sig precomputed_coordinates] in *.
-    lazy match beta delta [m1add_precomputed_coordinates coordinates proj1_sig].
-    destruct_head' prod.
-    congruence.
-  }
-  (* Safety: memory is what it should be *)
-  ecancel_assumption.
+  lazy beta match zeta delta [m1add_precomputed_coordinates projective_repr precomputed_coordinates coordinates proj1_sig].
+  unshelve eexists.
+  eexists (_, _, _, _, _).
+  2: solve_mem.
+  ssplit; try solve_bounds.
+  lazy [bin_model bin_add bin_mul bin_sub] in *. congruence.
 Qed.
 
 Lemma double_ok : program_logic_goal_for_function! double.
@@ -473,79 +470,39 @@ Proof.
   Strategy -1000 [un_xbounds bin_xbounds bin_ybounds un_square bin_mul bin_add bin_carry_add bin_sub bin_carry_sub un_outbounds bin_outbounds].
 
   straightline.
-  destruct a0 as ((((fx, fy), fz), fta), ftb).
-  destruct p as (((((x, y), z), ta), tb), HP).
-  destruct anything as ((((ax, ay), az), ata), atb).
-  lazy beta match delta [point_repr_bounded_by feval_point_repr coordinates proj1_sig] in *.
-  repeat straightline.
-  inversion H13.
+  destruct_points.
+
   repeat single_step.
 
   (* Solve the postconditions *)
   repeat straightline.
-
   solve_deallocation.
-
-  eexists (_, _, _, _, _); ssplit; try ecancel_assumption; try solve_bounds.
-  lazy [bin_model bin_mul bin_add bin_carry_add bin_sub bin_carry_sub un_model un_square] in *.
-  lazy match zeta beta delta [m1double coordinates proj1_sig].
+  lazy beta match zeta delta [projective_repr coordinates proj1_sig m1double bin_model bin_add bin_mul bin_sub bin_carry_add bin_sub bin_carry_sub un_model un_square] in *.
+  unshelve eexists.
+  eexists (_, _, _, _, _).
+  2: solve_mem.
+  ssplit; try solve_bounds.
   rewrite F.pow_2_r in *.
-  congruence.
-Qed.
-
-Lemma to_cached_ok: program_logic_goal_for_function! to_cached.
-Proof.
-  repeat single_step. repeat straightline.
-  
-  exists x1, x3, z, x5; ssplit; try solve_bounds; try solve_mem.
-  
-  destruct p. 
-  cbv [bin_model bin_mul bin_add bin_carry_add bin_sub coordinates proj1_sig] in *.
-  cbv match beta delta [m1_prep cached_coordinates proj1_sig].
-  rewrite H31, H28, H26, H22, H20, H16.
-  simpl. rewrite H6. auto.
-
-    (* Without this, resolution of cbv stalls out Qed. *)
-  Strategy -1000 [un_xbounds bin_xbounds bin_ybounds un_square bin_model cached_coordinates proj1_sig bin_mul bin_add bin_carry_add bin_sub un_outbounds bin_outbounds].
+  Prod.inversion_prod. congruence.
 Qed.
 
 Lemma readd_ok : program_logic_goal_for_function! readd.
 Proof.
-  repeat single_step. repeat straightline_cleanup.
-
-  exists l5. split.
- - simpl. reflexivity. (* Local variables *)
- - cbv [FElem] in *.
-
- (* Prove the deallocation. Rewrite the last stack to byte representation and remember output variable names for later. *)
-  remember (Bignum.Bignum felem_size_in_words oxK _) as Ox in H92.
-  remember (Bignum.Bignum felem_size_in_words oyK _) as Oy in H92.
-  remember (Bignum.Bignum felem_size_in_words ozK _) as Oz in H92.
-  remember (Bignum.Bignum felem_size_in_words otaK _) as Ota in H92.
-  remember (Bignum.Bignum felem_size_in_words otbK _) as Otb in H92.
-  do 6 (seprewrite_in @Bignum.Bignum_to_bytes H92).
-  subst Ox Oy Oz Ota Otb.
-  extract_ex1_and_emp_in H92.
-  (* Now the hypothesis is in a format that straightline can solve. *)
-  repeat straightline.
-
-  (* Bounds *)
-  exists x10, x11, x12, x6, x9.
-  ssplit; solve_bounds.
-
-  (* Correctness *)
-  cbv [bin_model bin_mul bin_add bin_carry_add bin_sub] in *.
-  cbv match beta delta [m1_readd coordinates proj1_sig].
-  (* Get the elements out of c and p *)
-  destruct p. cbv match beta delta [coordinates proj1_sig] in H13. rewrite H13.
-  destruct c. cbv match beta delta [cached_coordinates proj1_sig] in H19. rewrite H19.
-  congruence.
-
-  (* Memory after program execution. *)
-  ecancel_assumption.
-
   (* Without this, resolution of cbv stalls out Qed. *)
-  Strategy -1000 [un_xbounds bin_xbounds bin_ybounds un_square bin_mul bin_add bin_carry_add bin_sub un_outbounds bin_outbounds].
+  Strategy -1000 [un_xbounds bin_xbounds bin_ybounds un_square bin_mul bin_add bin_carry_add bin_sub bin_carry_sub un_outbounds bin_outbounds].
+
+  straightline.
+  destruct_points.
+
+  repeat single_step. repeat straightline.
+
+  solve_deallocation.
+
+  unshelve eexists.
+  eexists (_, _, _, _, _). 2: solve_mem.
+  lazy match beta zeta delta [m1_readd coordinates proj1_sig bin_model bin_mul bin_add bin_carry_add bin_sub] in *.
+  ssplit; try solve_bounds.
+  Prod.inversion_prod. congruence.
 Qed.
 
 End WithParameters.
